---
title: "Base Case Behavior."
author: "Giordano Rogers"
date: "2025-01-02"
categories: [programming, philosophy]
image: "image.jpg"
---
# Base Case Behavior

The concept of base cases in inductive hypotheses are a good way to approach
programming.

Always test the base case: the most simple version of what you're trying to 
achieve.

You want to build a wrapper around an api?

Make the simplest possible api call first.

You want to build your own REST API to interact with your database?

Build one that prints a simple "hello world" response first.

Alwasy start simple.

Always start with the base case.

From there, you have a foundation to reason about the rest of the sequence.

Now I have a frame.

If I add this one small next step, I can it again.

I can keep iterating slowly through the sequence of events until I reach the 
outcome I'm looking for.

But now I'm not looking blindly.

Base case programming is prototyping.

But unlike the concept of protoyping, the term base case programming emphasizes
two important things. First, is simplicity. In mathematical reasoning, the base
case is always considered somewhat arbitrary, usually contained withing the
definition of the proposition itself. 

Consider the following sequence:
$$
x_n = 2x_{n-1} + x_{n-2} \quad \text{for} \quad n \geq 3
$$

Use induction to prove that $a_{2n}$ is even for all integers $n \ge 1$.

When you first see a prolem like this, there's no clear way to reason about.

Now, if I give you the start of the sequence, you can start to build up an intuition.

$$
x_1 = -1, \quad x_2 = 0, \quad x_n = 2x_{n-1} + x_{n-2} \quad \text{for} \quad n \geq 3
$$

The way we'd prove the conjecture formally, is by starting with these base cases, and reasoning up.

$$
x_3 = 2(0) + (-1) = -1
x_4 = 2(-1) + (0) = -2
x_5 = 2(-2) + (-1) = -5
$$

But to prove the statement generally, we don't have to show every step of the sequence.

We just have to show that the next step always follows the same pattern.

Assume that $x_{2k}$ is even for some integer $k \ge 1$. We can prove that $x_2(k+1)$ is even, because:

$$
x_{2(k+1)} = 2x_{2(k+1)-1} + x_{2(k+1)-2} = 2x_{k+1} + a_{2k}
$$

Since $a_{2k}$ is even, and $2a_{2k+1} must be even sice $a_{2K+1} 

In this example, there


The base case is always 